xtext/org.archware.sosadl/src/org/archware/sosadl/validation/typing/impl/CellEnvironmentImpl.java
@@ -1,5 +1,9 @@
 package org.archware.sosadl.validation.typing.impl;
 
+import java.util.function.BiFunction;
+import java.util.function.Supplier;
+import java.util.stream.Stream;
+
 import org.archware.sosadl.validation.typing.EnvContent;
 import org.archware.sosadl.validation.typing.Environment;
 
@@ -33,5 +37,15 @@ public class CellEnvironmentImpl extends EnvironmentImpl implements Environment 
 	
 	public Environment getParent() {
 		return parent;
+	}
+
+	@Override
+	public Stream<EnvContent> stream() {
+		return Stream.concat(Stream.of(info), parent.stream());
+	}
+
+	@Override
+	public <T> T match(BiFunction<EnvContent, Environment, T> ifCons, Supplier<T> ifNil) {
+		return ifCons.apply(info, parent);
 	}
 }
