xtext/org.archware.sosadl/src/org/archware/sosadl/validation/typing/impl/EnvironmentImpl.java
@@ -1,5 +1,9 @@
 package org.archware.sosadl.validation.typing.impl;
 
+import java.util.function.BiFunction;
+import java.util.function.Supplier;
+import java.util.stream.Stream;
+
 import org.archware.sosadl.validation.typing.EnvContent;
 import org.archware.sosadl.validation.typing.Environment;
 
@@ -14,4 +18,13 @@ public class EnvironmentImpl implements Environment {
 		return new CellEnvironmentImpl(this, name, info);
 	}
 
+	@Override
+	public Stream<EnvContent> stream() {
+		return Stream.empty();
+	}
+
+	@Override
+	public <T> T match(BiFunction<EnvContent, Environment, T> ifCons, Supplier<T> ifNil) {
+		return ifNil.get();
+	}
 }
